Main.lean
@@ -3,31 +3,58 @@ import LeanSorting.PartialFin
 import LeanSorting.PartialFinUnsafe
 import LeanSorting.PartialUSizeUnsafe
 
-def getLines : IO (Array String) := do
-  let stdin ← IO.getStdin
-  let mut lines : Array String := #[]
-  let mut currLine ← stdin.getLine
-  while !currLine.isEmpty do
-    -- Drop trailing newline
-    lines := lines.push (currLine.dropRight 1)
-    currLine ← stdin.getLine
-  pure lines
+-- def String.splitByLines (s : String) : Array String :=
+--   s.split (· == '\n') |>.toArray
 
-def mainSort (sort : Array String → Array String) : IO Unit := do
-  let lines ← getLines
-  let mut count := 0
-  for line in sort lines do
-    -- IO.println line
-    count := count + line.length
-  IO.println count
+#check String.get
+#check String.push
+#check Lean.TraceData
+#check IO.FS.SystemTime.nsec
 
-def main (args : List String) : IO UInt32 := do
-  match args with
-  -- | ["--mergeSort"] => mainSort Array.mergeSort; pure 0
-  | ["--mergeSortPartialFin"] => mainSort Array.mergeSortPartialFin; pure 0
-  | ["--mergeSortPartialFinUnsafe"] => mainSort Array.mergeSortPartialFinUnsafe; pure 0
-  | ["--mergeSortPartialUSizeUnsafe"] => mainSort Array.mergeSortPartialUSizeUnsafe; pure 0
-  | ["--qsort"] => mainSort (Array.qsort · (· < ·)); pure 0
-  | _ =>
-    IO.println "Expected single argument, either \"--msort\" or \"--qsort\""
+-- def String.toInt
+
+def main : List String → IO UInt32
+  | "--algorithm" :: algorithm :: "--files" :: files => do
+    let filesLines : List (Array UInt64) ← files.mapM fun file => do
+      let nats := (← IO.FS.lines ⟨file⟩).map fun str =>
+        let nat := str.toNat!
+        UInt64.ofNat nat
+      pure nats
+    -- let filesLines : List (Array Nat) := filesLines.map (·.map String.toNat!)
+    let mut aux := #[]
+    for lines in filesLines do
+      let start ← IO.monoMsNow
+      match algorithm with
+      -- | "Array.mergeSort" => sorry
+      | "Array.qsortOrd" =>
+        let mut sum := 0
+        for line in lines.qsortOrd do
+          sum := sum + line
+        println! "sum = {sum}"
+      | "Array.mergeSortPartialFin" =>
+        let mut sum := 0
+        for line in lines.mergeSortPartialFin do
+          sum := sum + line
+        println! "sum = {sum}"
+      | "Array.mergeSortPartialFinUnsafe" =>
+        let mut sum := 0
+        for line in lines.mergeSortPartialFinUnsafe do
+          sum := sum + line
+        println! "sum = {sum}"
+      | "Array.mergeSortPartialFinUnsafeAux" =>
+        let mut sum := 0
+        let mut lines := lines
+        (lines, aux) := lines.mergeSortPartialFinUnsafe' aux
+        for line in lines do
+          sum := sum + line
+        println! "sum = {sum}"
+      | _ =>
+        println! "unknown algorithm: {algorithm}"
+        return 1
+      let endTime ← IO.monoMsNow
+      let elapsed := endTime - start
+      println! "elapsed = {elapsed}"
+    pure 0
+  | _ => do
+    println! "Usage: --algorithm <ALGO> --files <FILE> ..."
     pure 1
