profile.sh
@@ -1,9 +1,11 @@
 #!/usr/bin/env bash
 
+FILES=$@
+
 profile() {
     echo "Testing $1"
     for _ in {1..10}; do
-        { time ./.lake/build/bin/lsort --"$1" < ./test-input/1-million-lines.txt > /dev/null ; } 2>&1 \
+        { time ./.lake/build/bin/lsort $@ --files $FILES > /dev/null ; } 2>&1 \
             | head -2 \
             | tail -1
     done
@@ -11,7 +13,9 @@ profile() {
 
 lake build lsort
 
-profile mergeSortPartialFin
-profile mergeSortPartialFinUnsafe
-profile mergeSortPartialUSizeUnsafe
-profile qsort
+profile --algorithm Array.mergeSortPartialFinUnsafe\\'
+profile --algorithm Array.qsortOrd
+profile --algorithm Array.mergeSortPartialFin
+# profile --algorithm Array.mergeSortPartialUSizeUnsafe
+# profile --algorithm Array.mergeSortPartialUSizeUnsafe\\'
+# profile --algorithm qsort
